added Example

src/AST.v
@@ -12,21 +12,6 @@ Definition ident := Z.
 Definition BitV (n : nat) : Type := (@Integers.Int n).
 
 
-(* (* Do we need anything with this? *) *)
-(* Inductive NumInfo := *)
-(* (*| BinLit (n : nat) *)
-(* | OctLit (n : nat) *) *)
-(* | DecLit *)
-(* (*| HexLit (n : nat) *)
-(* | CharLit *)
-(* | PolyLit (n : nat)*) *)
-(* . *)
-
-(* Inductive Literal := *)
-(* | ECNum (n : nat) (inf : NumInfo) *)
-(* (* | ECString (s : string)*) *)
-(* . *)
-
 
 Inductive Selector :=
 | TupleSel (n : nat) (o : option nat)
@@ -79,6 +64,7 @@ with DeclGroup :=
 .
 
 (* TODO: make sure we can shadow variables 5 and 6 here, or change up *)
+(* Pretty sure this just works, due to eager evaluation order *)
 Definition builtin_binop (id : ident) (op : binop) : DeclGroup :=
   NonRecursive (Decl id (DExpr (EAbs 5 (EAbs 6 (EBinop op (EVar 5) (EVar 6)))))).
 
@@ -115,6 +101,7 @@ Inductive val :=
 | vcons (v : val) (e : Expr) (E : ident -> option val) (* lazy list: first val computed, rest is thunked *)
 | vnil (* empty list *)
 | tuple (l : list val) (* heterogeneous tuples *)
+
 .
 
 Definition env := ident -> option val.
@@ -250,7 +237,6 @@ Inductive eval_expr (ge : genv) : env -> Expr -> val -> Prop :=
       eval_expr E (EListSel lst idx) v*)
 
 
-(* Haskell Tests *)
 
 (* Verbatim ASTs from cryptol: *)
 (* First we need some list notation to match Haskell *)
@@ -263,114 +249,4 @@ Definition  Nothing {A : Type} : option A := None.
 End HaskellListNotations.
 
 Import HaskellListNotations.
-
-(* right side of this generated from cryptol implementation *)
-
-Definition id_cry : DeclGroup := (NonRecursive (Decl 242 (DExpr (EAbs 243 (EWhere (EApp (EVar 244) (EVar 243)) [(Recursive [(Decl 244 (DExpr (EAbs 245 (EIf (EApp (EApp (EVar 17) (EVar 245)) (EVar 0)) (EVar 0) (EApp (EApp (EVar 1) (EVar 0)) (EApp (EVar 244) (EApp (EApp (EVar 1) (EVar 245)) (EApp (EVar 11) (EVar 0)))))))))])]))))).
-
-Definition width : nat := 32.
-
-Lemma nz :
-  width <> O.
-Proof.
-  unfold width. congruence.
-Qed.
-
-Definition lit (z : Z) : Expr :=
-  ELit (@repr width nz z).
-
-(* 17 -> eq *)
-(* 1 -> plus *)
-Definition id_cry_hand_mod : DeclGroup := (NonRecursive (Decl 242 (DExpr (EAbs 243 (EWhere (EApp (EVar 244) (EVar 243)) [(Recursive [(Decl 244 (DExpr (EAbs 245 (EIf (EApp (EApp (EVar 17) (EVar 245)) (lit 0)) (lit 0) (EApp (EApp (EVar 1) (lit 1)) (EApp (EVar 244) (EApp (EApp (EVar 1) (EVar 245)) (lit (-1)))))))))])]))))).
-
-Definition eq_decl := builtin_binop 17 Eq.
-Definition plus_decl := builtin_binop 1 Plus.
-
-Definition id_ge := bind_decl_group id_cry_hand_mod
-                                    (bind_decl_group eq_decl
-                                                     (bind_decl_group plus_decl gempty)).
-Definition E := extend empty 12 (bits (@repr width nz 2)).
-
-Lemma eval_id :
-  eval_expr id_ge E (EApp (EVar 242) (EVar 12)) (bits (@repr width nz 2)).
-Proof.
-  econstructor. unfold id_ge.
-  simpl. eapply eval_global_var. unfold E. unfold extend. simpl. unfold empty. auto.
-  simpl. reflexivity.
-  econstructor. econstructor. unfold E. unfold extend. simpl. reflexivity.
-  econstructor.
-  simpl. econstructor.
-  eapply eval_global_var. unfold E. unfold extend. simpl. unfold empty. auto.
-  simpl. reflexivity.
-  econstructor. econstructor. unfold extend. simpl. reflexivity.
-  eapply eval_if_f.
-  econstructor. econstructor.
-  eapply eval_global_var. unfold E. unfold extend. simpl. unfold empty. auto.
-  simpl. unfold id_ge. unfold bind_decl_group. simpl. reflexivity.
-  econstructor; eauto.
-  econstructor; eauto. unfold extend. simpl. reflexivity.
-  econstructor; eauto.
-  econstructor; eauto.
-  econstructor; eauto.
-  econstructor; eauto. unfold extend. simpl. reflexivity.
-  econstructor; eauto. unfold extend. simpl. reflexivity.
-  econstructor; eauto; exact nz.
-
-  econstructor. econstructor. eapply eval_global_var. unfold E. unfold extend. simpl. unfold empty. reflexivity.
-  simpl. unfold id_ge. simpl. reflexivity.
-
-  econstructor. econstructor; eauto.
-  econstructor; eauto.
-  econstructor; eauto.
-  eapply eval_global_var; eauto. simpl. reflexivity.
-  econstructor; eauto.
-  econstructor. econstructor.
-  eapply eval_global_var; eauto. simpl. unfold id_ge. simpl. reflexivity.
-  econstructor. econstructor.
-  unfold extend. simpl. reflexivity.
-  econstructor. econstructor. econstructor. econstructor.
-  unfold extend. simpl. reflexivity.
-  econstructor. unfold extend. simpl. reflexivity.
-  econstructor. exact nz.
-
-  eapply eval_if_f. econstructor.
-  econstructor. eapply eval_global_var; eauto. simpl. unfold id_ge. simpl. reflexivity.
-  econstructor. econstructor. unfold E. unfold extend. simpl. reflexivity.
-
-  econstructor. econstructor.
-  econstructor;
-    try econstructor; try unfold extend; simpl; eauto.
-  econstructor; exact nz.
-  
-  econstructor.
-  econstructor. eapply eval_global_var; eauto. simpl. unfold id_ge. simpl. reflexivity.
-  econstructor. econstructor.
-  econstructor. econstructor.
-  eapply eval_global_var. simpl. unfold id_ge. simpl. reflexivity. simpl. reflexivity.
-  econstructor. econstructor. econstructor. eapply eval_global_var.
-  simpl. unfold id_ge. simpl. reflexivity. simpl. reflexivity.
-  econstructor. econstructor. unfold extend. simpl. reflexivity.
-  econstructor. econstructor.
-  econstructor. econstructor. unfold extend. simpl. reflexivity.
-  econstructor. unfold extend. simpl. reflexivity.
-  econstructor. exact nz.
-  eapply eval_if_t. econstructor. econstructor.
-  eapply eval_global_var. unfold extend. simpl. unfold E. unfold extend. simpl. unfold empty.
-  reflexivity.
-  simpl. unfold id_ge. simpl. reflexivity.
-  econstructor. econstructor. unfold extend. simpl. reflexivity.
-  econstructor. econstructor. econstructor; try unfold extend; try econstructor; simpl; eauto.
-  econstructor; eauto; exact nz.
-  econstructor.
-  econstructor. econstructor. unfold extend. simpl. reflexivity.
-  econstructor. unfold extend. simpl. reflexivity.
-  econstructor. exact nz.
-  econstructor. econstructor. unfold extend. simpl. reflexivity.
-  econstructor. unfold extend. simpl. reflexivity.
-  econstructor. exact nz.
-  Unshelve.
-  all: exact nz.
-Qed.
-  
-
 
